Examples.thy
@@ -1,5 +1,5 @@
 theory Examples
-imports DerivedCombinators PartialEvaluation
+imports DerivedCombinators PartialEvaluation Typechecking
 begin
 
 definition is_zero_expr :: expr where
@@ -21,60 +21,20 @@ definition greater_than_expr :: expr where
 definition length_expr :: "type \<Rightarrow> expr" ("length\<^bsub>_\<^esub>") where
   "length\<^bsub>t\<^esub> = \<lparr> \<kappa> ZeroV \<nabla> (succ \<cdot> \<pi>\<^sub>2) \<rparr>\<^bsub>ListF t\<^esub>"
 
-lemma [simp]: "is_zero_expr \<turnstile> Nat \<rightarrow> Bool"
-  proof (unfold is_zero_expr_def)
-    have "\<prec>\<^bsub>NatF\<^esub> \<turnstile> Nat \<rightarrow> Nat \<star> NatF" by (metis tc_outj)
-    hence "\<prec>\<^bsub>NatF\<^esub> \<turnstile> Nat \<rightarrow> \<one> \<oplus> Nat" by simp
-    moreover have "\<epsilon> \<bar> \<kappa> UnitV \<turnstile> \<one> \<oplus> Nat \<rightarrow> Bool" by simp
-    ultimately show "\<epsilon> \<bar> \<kappa> UnitV \<cdot> \<prec>\<^bsub>NatF\<^esub> \<turnstile> Nat \<rightarrow> Bool" by (metis tc_comp)
-  qed
+lemma "algorithmic_typecheck is_zero_expr = Some (Nat \<hookrightarrow> Bool)"
+  by (simp add: is_zero_expr_def Let_def)
 
-lemma [simp]: "pred_expr \<turnstile> Nat \<rightarrow> Nat"
-  proof (unfold pred_expr_def)
-    have "\<prec>\<^bsub>NatF\<^esub> \<turnstile> Nat \<rightarrow> Nat \<star> NatF" by (metis tc_outj)
-    hence "\<prec>\<^bsub>NatF\<^esub> \<turnstile> Nat \<rightarrow> \<one> \<oplus> Nat" by simp
-    moreover have "\<kappa> ZeroV \<nabla> \<epsilon> \<turnstile> \<one> \<oplus> Nat \<rightarrow> Nat" by simp
-    ultimately show "\<kappa> ZeroV \<nabla> \<epsilon> \<cdot> \<prec>\<^bsub>NatF\<^esub> \<turnstile> Nat \<rightarrow> Nat" by (metis tc_comp)
-  qed
+lemma [simp]: "algorithmic_typecheck pred_expr = Some (Nat \<hookrightarrow> Nat)"
+  by (simp add: pred_expr_def Let_def)
 
-lemma [simp]: "greater_than_helper \<turnstile> Nat \<otimes> Nat \<rightarrow> Bool \<oplus> Nat \<otimes> Nat"
-  proof (unfold greater_than_helper_def)
-    have E: "is_zero_expr \<turnstile> Nat \<rightarrow> Bool" by simp
-    moreover have "\<pi>\<^sub>1 \<turnstile> Nat \<otimes> Nat \<rightarrow> Nat" by simp
-    ultimately have X: "is_zero_expr \<cdot> \<pi>\<^sub>1 \<turnstile> Nat \<otimes> Nat \<rightarrow> Bool" by (metis tc_comp)
-    have I: "\<iota>\<^sub>l \<turnstile> Bool \<rightarrow> Bool \<oplus> Nat \<otimes> Nat" by simp
-    moreover have "\<kappa> FalseV \<turnstile> Nat \<otimes> Nat \<rightarrow> Bool" by simp
-    ultimately have Y: "\<iota>\<^sub>l \<cdot> \<kappa> FalseV \<turnstile> Nat \<otimes> Nat \<rightarrow> Bool \<oplus> Nat \<otimes> Nat" by (metis tc_comp)
-    have "\<pi>\<^sub>2 \<turnstile> Nat \<otimes> Nat \<rightarrow> Nat" by simp
-    with E have Z: "is_zero_expr \<cdot> \<pi>\<^sub>2 \<turnstile> Nat \<otimes> Nat \<rightarrow> Bool" by (metis tc_comp)
-    have "\<kappa> TrueV \<turnstile> Nat \<otimes> Nat \<rightarrow> Bool" by simp
-    with I have W: "\<iota>\<^sub>l \<cdot> \<kappa> TrueV  \<turnstile> Nat \<otimes> Nat \<rightarrow> Bool \<oplus> Nat \<otimes> Nat" by (metis tc_comp)
-    have "pred_expr \<parallel> pred_expr \<turnstile> Nat \<otimes> Nat \<rightarrow> Nat \<otimes> Nat" by simp
-    moreover have "\<iota>\<^sub>r \<turnstile> Nat \<otimes> Nat \<rightarrow> Bool \<oplus> Nat \<otimes> Nat" by simp
-    ultimately have "\<iota>\<^sub>r \<cdot> pred_expr \<parallel> pred_expr \<turnstile> Nat \<otimes> Nat \<rightarrow> Bool \<oplus> Nat \<otimes> Nat" by (metis tc_comp)
-    with X Y Z W show "
-      IF is_zero_expr \<cdot> \<pi>\<^sub>1 THEN \<iota>\<^sub>l \<cdot> \<kappa> FalseV 
-      ELSE IF is_zero_expr \<cdot> \<pi>\<^sub>2 THEN \<iota>\<^sub>l \<cdot> \<kappa> TrueV 
-      ELSE \<iota>\<^sub>r \<cdot> pred_expr \<parallel> pred_expr 
-      FI FI 
-        \<turnstile> Nat \<otimes> Nat \<rightarrow> Bool \<oplus> Nat \<otimes> Nat" by simp
-  qed
+lemma [simp]: "algorithmic_typecheck greater_than_helper = Some (Nat \<otimes> Nat \<hookrightarrow> Bool \<oplus> Nat \<otimes> Nat)"
+  by (simp add: greater_than_helper_def pred_expr_def is_zero_expr_def Let_def)
 
-lemma "greater_than_expr \<turnstile> Nat \<otimes> Nat \<rightarrow> Bool"
-  proof (unfold greater_than_expr_def)
-    have "\<lparr> \<Xi> \<rparr>\<^bsub>K Bool \<Oplus> funct.Id\<^esub> \<turnstile> \<mu> (K Bool \<Oplus> Id) \<rightarrow> Bool" by simp
-    moreover have "\<lbrakk> greater_than_helper \<rbrakk>\<^bsub>K Bool \<Oplus> Id\<^esub> \<turnstile> Nat \<otimes> Nat \<rightarrow> \<mu> (K Bool \<Oplus> Id)" by simp
-    ultimately show "\<lparr> \<Xi> \<rparr>\<^bsub>K Bool \<Oplus> funct.Id\<^esub> \<cdot> \<lbrakk> greater_than_helper \<rbrakk>\<^bsub>K Bool \<Oplus> Id\<^esub> 
-      \<turnstile> Nat \<otimes> Nat \<rightarrow> Bool" by (metis tc_comp)
-  qed
+lemma "algorithmic_typecheck greater_than_expr = Some (Nat \<otimes> Nat \<hookrightarrow> Bool)"
+  by (simp add: greater_than_expr_def greater_than_helper_def pred_expr_def is_zero_expr_def Let_def)
 
-lemma "length\<^bsub>t\<^esub> \<turnstile> List t \<rightarrow> Nat"
-  proof (unfold length_expr_def)
-    have "succ \<turnstile> Nat \<rightarrow> Nat" by simp
-    moreover have "\<pi>\<^sub>2 \<turnstile> t \<otimes> Nat \<rightarrow> Nat" by simp
-    ultimately have "succ \<cdot> \<pi>\<^sub>2 \<turnstile> t \<otimes> Nat \<rightarrow> Nat" by (metis tc_comp)
-    thus "\<lparr> \<kappa> ZeroV \<nabla> (succ \<cdot> \<pi>\<^sub>2) \<rparr>\<^bsub>ListF t\<^esub> \<turnstile> List t \<rightarrow> Nat" by simp
-  qed
+lemma "algorithmic_typecheck length\<^bsub>t\<^esub> = Some (List t \<hookrightarrow> Nat)"
+  by (simp add: length_expr_def )
 
 primrec nat_to_val :: "nat \<Rightarrow> val" where
   "nat_to_val 0 = ZeroV"
